update if dataset

src/If/CommonLemmas.v
@@ -3,6 +3,10 @@ From Hammer Require Import Tactics Hammer.
 Require Import UrsusEnvironment.Solidity.current.Environment.
 Require Import SpecLang.
 
+Require Import If.If.
+Import If.
+Require Import If.Common.
+
 Fixpoint reference_hash_implementation 
     (n: nat)
         (m_string: uint64[])
@@ -22,3 +26,64 @@ Fixpoint reference_hash_implementation
         let pw' := N.modulo (pw * m_multiplier) m_modulo in
         (h', pw', false)
     end.
+
+
+Definition hash_1_correct_def (ll: LedgerLRecord rec) : Prop.
+execs0 (hash_1 rec def) :
+ll | "m_string" "m_modulo" "m_multiplier" -> l1 | "m_hash".
+con (m_hash = fst (fst (reference_hash_implementation 1%nat m_string (uint2N m_multiplier) (uint2N m_modulo)))).
+Defined.
+
+Definition hash_2_correct_def (ll: LedgerLRecord rec) : Prop.
+execs0 (hash_2 rec def) :
+ll | "m_string" "m_modulo" "m_multiplier" -> l1 | "m_hash".
+con (m_hash = fst (fst (reference_hash_implementation 2%nat m_string (uint2N m_multiplier) (uint2N m_modulo)))).
+Defined.
+
+Definition hash_3_correct_def (ll: LedgerLRecord rec) : Prop.
+execs0 (hash_3 rec def) :
+ll | "m_string" "m_modulo" "m_multiplier" -> l1 | "m_hash".
+con (m_hash = fst (fst (reference_hash_implementation 3%nat m_string (uint2N m_multiplier) (uint2N m_modulo)))).
+Defined.
+
+Definition hash_4_correct_def (ll: LedgerLRecord rec) : Prop.
+execs0 (hash_4 rec def) :
+ll | "m_string" "m_modulo" "m_multiplier" -> l1 | "m_hash".
+con (m_hash = fst (fst (reference_hash_implementation 4%nat m_string (uint2N m_multiplier) (uint2N m_modulo)))).
+Defined.
+
+Definition hash_5_correct_def (ll: LedgerLRecord rec) : Prop.
+execs0 (hash_5 rec def) :
+ll | "m_string" "m_modulo" "m_multiplier" -> l1 | "m_hash".
+con (m_hash = fst (fst (reference_hash_implementation 5%nat m_string (uint2N m_multiplier) (uint2N m_modulo)))).
+Defined.
+
+Definition hash_6_correct_def (ll: LedgerLRecord rec) : Prop.
+execs0 (hash_6 rec def) :
+ll | "m_string" "m_modulo" "m_multiplier" -> l1 | "m_hash".
+con (m_hash = fst (fst (reference_hash_implementation 6%nat m_string (uint2N m_multiplier) (uint2N m_modulo)))).
+Defined.
+
+Definition hash_7_correct_def (ll: LedgerLRecord rec) : Prop.
+execs0 (hash_7 rec def) :
+ll | "m_string" "m_modulo" "m_multiplier" -> l1 | "m_hash".
+con (m_hash = fst (fst (reference_hash_implementation 7%nat m_string (uint2N m_multiplier) (uint2N m_modulo)))).
+Defined.
+
+Definition hash_8_correct_def (ll: LedgerLRecord rec) : Prop.
+execs0 (hash_8 rec def) :
+ll | "m_string" "m_modulo" "m_multiplier" -> l1 | "m_hash".
+con (m_hash = fst (fst (reference_hash_implementation 8%nat m_string (uint2N m_multiplier) (uint2N m_modulo)))).
+Defined.
+
+Definition hash_9_correct_def (ll: LedgerLRecord rec) : Prop.
+execs0 (hash_9 rec def) :
+ll | "m_string" "m_modulo" "m_multiplier" -> l1 | "m_hash".
+con (m_hash = fst (fst (reference_hash_implementation 9%nat m_string (uint2N m_multiplier) (uint2N m_modulo)))).
+Defined.
+
+Definition hash_10_correct_def (ll: LedgerLRecord rec) : Prop.
+execs0 (hash_10 rec def) :
+ll | "m_string" "m_modulo" "m_multiplier" -> l1 | "m_hash".
+con (m_hash = fst (fst (reference_hash_implementation 10%nat m_string (uint2N m_multiplier) (uint2N m_modulo)))).
+Defined.
