src/If/CommonContractTactics.v
@@ -1,4 +1,5 @@
 Require Export CommonTactics.
+Require Import UrsusEnvironment.Solidity.current.Environment.
 
 Require Import If.If.
 Import If.
@@ -32,4 +33,129 @@ Ltac preprocess_ifs :=
       end
   end.
 
-Ltac bottom_up_goal_solver' := preprocess_ifs; bottom_up_goal_solver.
+  Ltac lift_lets P0 Heql Hprev :=
+    (* repeat *) match goal with
+    | |- P0 ?ll => 
+        match ll with
+        | (let x:=?t in @?f x) =>
+            idtac "'let' is found in the goal with:" x;
+            match goal with
+            | _ =>  idtac "item is not found, making new for" t;
+                    let y := fresh "y" in
+                    pose (y:=t);
+                    let f' := eval cbv beta in (f y) in
+                    change_no_check (P0 ll) with (P0 f');
+                    let H := fresh "H" in
+                    assert (y = t) as H by (* (exact_no_check eq_refl) *) reflexivity;
+                    clearbody y;
+                    move y before Hprev;
+                    move H before Hprev;
+                    lift_lets P0 Heql (H)
+            end
+        | _ => idtac "'let' is not found in the goal";
+               match goal with
+               | H: ?z = ll |- _ => idtac "item is found:" z;
+                                    change_no_check (P0 ll) with (P0 z)
+                                
+               | _ =>  idtac "item is not found, making new for" ll;
+                       let y := fresh "y" in
+                       pose (y:=ll);
+                       change_no_check (P0 ll) with (P0 y);
+                       let H := fresh "H" in
+                       assert (y = ll) as H by (* (exact_no_check eq_refl) *) reflexivity;
+                       clearbody y;  
+                       move y before Hprev;
+                       move H before Hprev
+               end;        
+               clear Heql;
+               subst P0; 
+               intros Heql;
+               match type of Heql with 
+                   | ?l = _ => subst l
+               end
+        end
+    end.
+
+Ltac continue f_exec f_exec_prf f_destructor Heql Hprev :=
+(* let Heql := fresh "Heql" in *)
+(* match goal with 
+| |- ?P _ =>  *)
+(* Heql = ? = exec_state ... *)
+revert Heql;
+erewrite <- (* ? *)f_exec_prf; [
+(* |- fun_exec... *)
+let ll := fresh "ll" in
+let ll' := fresh "ll'" in
+f_destructor ll ll'; (* ? *)
+(* ll = fun_exec, ll' := ll |- f (ll) *)
+change_no_check ll with ll';
+(* ll = fun_exec, ll' := ll |- f (ll')  *)
+revert ll';
+(* ll = fun_exec |- let ll' := ll in f (ll')  *)
+let P0 := fresh "P" in 
+match goal with
+| |- let ll' := _ in @?F ll' => (* remember F as P0 *)
+     let HF := fresh "HeqF" in 
+     pose F as P0; assert (P0 = F) as HF by (* (exact_no_check eq_refl) *)reflexivity; clearbody P0
+end;
+intros;
+(* ll = fun_exec, ll' := ll, P0 = |- P0 (ll')  *)
+(* match goal with
+| |- ?G => *) assert (P0 ll'); [| subst P0; (* subst P; *) auto]
+(* end *);
+subst ll' ll;
+cbv beta delta [f_exec];
+lift_lets P0 Heql Hprev | .. ].
+
+Ltac2 continue_iter x := 
+let t := ltac1:(p |- 
+idtac "looking for" p "in evals/execs";
+let continue_once a :=
+multimatch goal with
+| H: ?y = ?X |- _ => match X with
+                   | context [eval_state (UinterpreterUnf ?listInfinite ?t) ?l] =>
+                     match t with 
+                     | context [p] => 
+                       idtac "eval found" p "in" H "with" y;
+                       let h := eval cbn in ltac:(__index_hash p) in
+                       let ee := constr:(__eval (f:=h)) in
+                       let e := match ee with
+                       | @__eval _ _ _ _ ?I => eval cbv beta iota delta [__eval I] in ee
+                       end in
+                       (* let e := eval simpl __eval in (__eval (f:=p))in *)
+                       let d := ltac:(destructor_template e) in
+                       let eprf := constr:(__eval_prf (f:=h)) in
+                       let prf := match eprf with
+                       | @__eval_prf _ _ _ _ ?I => eval cbv beta iota delta [__eval_prf I] in eprf
+                       end in 
+                       continue e prf d H (y) 
+                     end   
+                   | context [exec_state (UinterpreterUnf ?listInfinite ?t) ?l] => 
+                     match t with 
+                     | context [p] =>
+                       idtac "exec found" p "in" H "with" y;
+                       let h := eval cbn in ltac:(__index_hash p) in
+                       let ee := constr:(__exec (f:=h)) in
+                       let e := match ee with
+                       | @__exec _ _ _ _ ?I => eval cbv beta iota delta [__exec I] in ee
+                       end in
+                       (* let e := eval simpl __exec in (__exec (f:=p))in *)
+                       let d := ltac:(destructor_template e) in
+                       let eprf := constr:(__exec_prf (f:=h)) in
+                       let prf := match eprf with
+                       | @__exec_prf _ _ _ _ ?I => eval cbv beta iota delta [__exec_prf I] in eprf
+                       end in
+                       continue e prf d H (y) 
+                     end
+                   (* | _ => idtac "no more" p "found in" H; fail *)
+                  end
+end in repeat2 continue_once) in t x.
+
+Tactic Notation "continue_all" constr_list(cl) :=
+idtac "Looking for list:" cl;
+let f := ltac2:(cl_raw |-
+let cl' := Option.get (Ltac1.to_list cl_raw) in
+List.iter (fun c => continue_iter c) cl') in 
+ f cl; (* simpl orb in * *) cbn [orb] in * . 
+ (* TODO: sometimes simpl orb simplifies orb in goal which is bad *)
+ (* Maybe cbn fixes that *)
