src/Main.v
@@ -1,7 +1,7 @@
 Require Import UrsusEnvironment.Solidity.current.Environment.
 
 Require Import Simple.Simple.
-(*Require Import If.If.*)
+Require Import If.If.
 Require Import Recursion.Recursion.
 (*Require Import IfAndRecursion.IfAndRecursion.*)
 
@@ -15,7 +15,7 @@ Elpi SetProjectRoot .
 Set Coq Root "src".
 
 Elpi GenerateCommon Simple "Simple" .
-(*Elpi GenerateCommon If "If" .*)
+Elpi GenerateCommon If "If" .
 Elpi GenerateCommon Recursion "Recursion" .
 (*Elpi GenerateCommon IfAndRecursion "IfAndRecursion" .*)
 
